floyd/entailer.v
@@ -1,0 +1,64 @@
+Require Import floyd.base.
+Require Import floyd.assert_lemmas.
+Require Import floyd.client_lemmas.
+Local Open Scope logic.
+
+
+Lemma and_solvable_left:
+ forall P Q : Prop,   P -> (P /\ Q) = Q.
+Proof. intros. apply prop_ext; intuition. Qed.
+
+Ltac and_solvable_left_aux1 :=
+  match goal with |- _ /\ _ => fail 1 | |- _ => solve [auto] end.
+
+Lemma and_solvable_right:
+ forall Q P : Prop,   Q -> (P /\ Q) = P.
+Proof. intros. apply prop_ext; intuition. Qed.
+
+Ltac and_solvable_left P :=
+ match P with
+  | ?P1 /\ ?P2 => try rewrite (and_solvable_left P1) by auto;
+                           and_solvable_left P2
+  | _ => match P with
+             | _ /\ _ => fail 1 
+             | _ => first [ rewrite (and_solvable_right P) by auto
+                                | rewrite (prop_true_andp' P) by auto
+                                | apply (prop_right P); solve [auto]
+                                | idtac
+                                ]
+             end
+  end.
+
+Ltac entailer' :=
+ autorewrite with gather_prop;
+ repeat ((simple apply go_lower_lem1 || apply derives_extract_prop || apply derives_extract_prop'); intro);
+ subst_any;
+ match goal with
+ |  |- _ |-- _ =>
+   saturate_local;  subst_any; 
+   change SEPx with SEPx'; unfold PROPx, LOCALx, SEPx', local, lift1;
+   unfold_lift; simpl;
+   autorewrite with gather_prop;
+   normalize;
+   autorewrite with gather_prop;
+   repeat rewrite and_assoc';
+   match goal with 
+   | |- _ |-- !! ?P && _ => and_solvable_left P
+   | |- _ |-- !! ?P => and_solvable_left P; 
+                               prop_right_cautious; try apply TT_right
+   | |- _ => idtac
+   end;
+   auto
+ | |- _ => normalize
+ end.
+
+Ltac entailer :=
+ match goal with
+ | |- PROPx _ _ |-- _ => 
+       go_lower; 
+       match goal with |- _ |-- _ => entailer' 
+                                 | |- _ => idtac 
+       end
+ | |- _ |-- _ => entailer'
+ | |- _ => fail "The entailer tactic works only on entailments   _ |-- _ "
+ end.
