floyd/proofauto.v
@@ -5,4 +5,8 @@ Require Export floyd.assert_lemmas.
 Require Export floyd.compare_lemmas.
 Require Export floyd.forward.
 Require Export floyd.malloc_lemmas.
+Require Export floyd.call_lemmas.
+Require Export floyd.forward_lemmas.
+Require Export floyd.loadstore_lemmas.
 Require Export floyd.array_lemmas.
+Require Export floyd.entailer.
